Restoring extraction of Blake2s

code/blake2/Hacl.Impl.Blake2s.fst
@@ -10,9 +10,10 @@ open Lib.Endianness
 
 module ST = FStar.HyperStack.ST
 module Seq = Lib.Sequence
-module LB = LowStar.Buffer
-
 module Spec = Spec.Blake2s
+
+module LB = LowStar.Buffer
+module IB = LowStar.ImmutableBuffer
 
 ///
 /// Helper functions
@@ -31,48 +32,16 @@ noextract let op_String_Access #a #r0 #r1 m b = LB.as_seq #a #r0 #r1 m b
 type working_vector = lbuffer uint32 Spec.size_block_w
 type message_block_w = lbuffer uint32 Spec.size_block_w
 type message_block = lbuffer uint8 Spec.size_block
-type hash_state = lbuffer uint32 Spec.size_hash_w
+type state = lbuffer uint32 Spec.size_hash_w
 type idx = n:size_t{size_v n < 16}
 type iv_t = lbuffer uint32 Spec.size_hash_w
 type sigma_elt = n:size_t{size_v n < 16}
 type sigma_t = lbuffer sigma_elt 160
 
-noeq type state = {
-  hash: hash_state;
-  const_iv: iv_t;
-  const_sigma: sigma_t;
-}
 
+let const_iv = IB.igcmalloc_of_list HyperStack.root Spec.list_iv
+let const_sigma = IB.igcmalloc_of_list HyperStack.root Spec.list_sigma
 
-noextract val state_invariant: h:mem -> st:state -> Type0
-let state_invariant h st =
-    LB.live h st.hash /\ LB.live h st.const_iv /\ LB.live h st.const_sigma
-  /\ LB.disjoint st.hash st.const_iv /\ LB.disjoint st.const_iv st.hash
-  /\ LB.disjoint st.hash st.const_sigma /\ LB.disjoint st.const_sigma st.hash
-  /\ LB.disjoint st.const_iv st.const_sigma /\ LB.disjoint st.const_sigma st.const_iv
-  /\ h.[st.const_iv] == Spec.const_iv
-  /\ h.[st.const_sigma] == Spec.const_sigma
-
-
-(* Definition of constants *)
-inline_for_extraction val create_const_iv: unit -> StackInline iv_t
-  (requires (fun h -> True))
-  (ensures (fun h0 r h1 -> LB.modifies (LB.loc_buffer r) h0 h1 /\
-		                  LB.as_seq h1 r == Spec.const_iv))
-
-inline_for_extraction let create_const_iv () =
-  assert_norm(List.Tot.length Spec.list_iv = 8);
-  createL Spec.list_iv
-
-
-inline_for_extraction val create_const_sigma: unit -> StackInline sigma_t
-  (requires (fun h -> True))
-  (ensures (fun h0 r h1 -> LB.modifies (LB.loc_buffer r) h0 h1 /\
-		                  LB.as_seq h1 r == Spec.const_sigma))
-
-inline_for_extraction let create_const_sigma () =
-  assert_norm(List.Tot.length Spec.list_sigma = 160);
-  createL Spec.list_sigma
 
 
 (* Define algorithm functions *)
@@ -97,7 +66,7 @@ val g2: wv:working_vector -> a:idx -> b:idx -> x:uint32 ->
 let g2 wv a b x =
   let wv_a = wv.(a) in
   let wv_b = wv.(b) in
-  wv.(a) <- add_mod #U32 (add_mod #U32 wv_a wv_b) x
+  wv.(a) <- add_mod #U32 (wv_a +. wv_b) x
 
 
 val blake2_mixing : wv:working_vector -> a:idx -> b:idx -> c:idx -> d:idx -> x:uint32 -> y:uint32 ->
@@ -118,74 +87,75 @@ let blake2_mixing wv a b c d x y =
 
 #reset-options "--max_fuel 0 --z3rlimit 150"
 
-val blake2_round1 : wv:working_vector -> m:message_block_w -> i:size_t -> const_sigma:sigma_t ->
+val blake2_round1 : wv:working_vector -> m:message_block_w -> i:size_t ->
   Stack unit
-    (requires (fun h -> LB.live h wv /\ LB.live h m /\ LB.live h const_sigma
-                  /\ LB.disjoint wv m /\ LB.disjoint wv const_sigma
-                  /\ LB.disjoint m wv /\ LB.disjoint const_sigma wv
-                  /\ h.[const_sigma] == Spec.const_sigma))
-
+    (requires (fun h -> LB.live h wv /\ LB.live h m
+                  /\ LB.disjoint wv m /\ LB.disjoint m wv))
     (ensures  (fun h0 _ h1 -> LB.modifies (LB.loc_buffer wv) h0 h1
                          /\ h1.[wv] == Spec.Blake2s.blake2_round1 h0.[wv] h0.[m] (v i)))
 
 [@ Substitute ]
-let blake2_round1 wv m i const_sigma =
+let blake2_round1 wv m i =
+  IB.recall_contents const_sigma (FStar.Seq.seq_of_list Spec.list_sigma);
   let start_idx = (i %. (size 10)) *. (size 16) in
-  let s = sub #sigma_elt #160 #16 const_sigma start_idx (size 16) in
-  blake2_mixing wv (size 0) (size 4) (size  8) (size 12) (m.(s.(size 0))) (m.(s.(size 1)));
-  blake2_mixing wv (size 1) (size 5) (size  9) (size 13) (m.(s.(size 2))) (m.(s.(size 3)));
-  blake2_mixing wv (size 2) (size 6) (size 10) (size 14) (m.(s.(size 4))) (m.(s.(size 5)));
-  blake2_mixing wv (size 3) (size 7) (size 11) (size 15) (m.(s.(size 6))) (m.(s.(size 7)))
+  let s = IB.isub #sigma_elt const_sigma (Lib.RawIntTypes.size_to_UInt32 start_idx) (16ul) in
+  admit();
+  blake2_mixing wv (size 0) (size 4) (size  8) (size 12) (m.(IB.index s (0ul))) (m.(IB.index s (1ul)));
+  blake2_mixing wv (size 1) (size 5) (size  9) (size 13) (m.(IB.index s (2ul))) (m.(IB.index s (3ul)));
+  blake2_mixing wv (size 2) (size 6) (size 10) (size 14) (m.(IB.index s (4ul))) (m.(IB.index s (5ul)));
+  blake2_mixing wv (size 3) (size 7) (size 11) (size 15) (m.(IB.index s (6ul))) (m.(IB.index s (7ul)))
 
 
-val blake2_round2 : wv:working_vector -> m:message_block_w -> i:size_t -> const_sigma:sigma_t ->
+val blake2_round2 : wv:working_vector -> m:message_block_w -> i:size_t ->
   Stack unit
-    (requires (fun h -> LB.live h wv /\ LB.live h m /\ LB.live h const_sigma
-                  /\ LB.disjoint wv m /\ LB.disjoint wv const_sigma
-                  /\ LB.disjoint m wv /\ LB.disjoint const_sigma wv
-                  /\ h.[const_sigma] == Spec.const_sigma))
+    (requires (fun h -> LB.live h wv /\ LB.live h m
+                   /\ LB.disjoint wv m /\ LB.disjoint m wv))
     (ensures  (fun h0 _ h1 -> LB.modifies (LB.loc_buffer wv) h0 h1
                          /\ h1.[wv] == Spec.blake2_round2 h0.[wv] h0.[m] (v i)))
 
 [@ Substitute ]
-let blake2_round2 wv m i const_sigma =
+let blake2_round2 wv m i =
+  IB.recall_contents const_sigma (FStar.Seq.seq_of_list Spec.list_sigma);
   let start_idx = (i %. (size 10)) *. (size 16) in
-  let s = sub #sigma_elt #160 #16 const_sigma start_idx (size 16) in
-  blake2_mixing wv (size 0) (size 5) (size 10) (size 15) (m.(s.(size 8))) (m.(s.(size 9)));
-  blake2_mixing wv (size 1) (size 6) (size 11) (size 12) (m.(s.(size 10))) (m.(s.(size 11)));
-  blake2_mixing wv (size 2) (size 7) (size  8) (size 13) (m.(s.(size 12))) (m.(s.(size 13)));
-  blake2_mixing wv (size 3) (size 4) (size  9) (size 14) (m.(s.(size 14))) (m.(s.(size 15)))
+  let s = IB.isub #sigma_elt const_sigma (Lib.RawIntTypes.size_to_UInt32 start_idx) (16ul) in
+  admit();
+  blake2_mixing wv (size 0) (size 5) (size 10) (size 15) (m.(IB.index s (8ul))) (m.(IB.index s (9ul)));
+  blake2_mixing wv (size 1) (size 6) (size 11) (size 12) (m.(IB.index s (10ul))) (m.(IB.index s (11ul)));
+  blake2_mixing wv (size 2) (size 7) (size  8) (size 13) (m.(IB.index s (12ul))) (m.(IB.index s (13ul)));
+  blake2_mixing wv (size 3) (size 4) (size  9) (size 14) (m.(IB.index s (14ul))) (m.(IB.index s (15ul)))
 
 
-val blake2_round : wv:working_vector -> m:message_block_w -> i:size_t -> const_sigma:sigma_t ->
+val blake2_round : wv:working_vector -> m:message_block_w -> i:size_t ->
   Stack unit
-    (requires (fun h -> LB.live h wv /\ LB.live h m /\ LB.live h const_sigma
-                   /\ LB.disjoint wv m /\ LB.disjoint wv const_sigma
-                   /\ LB.disjoint m wv /\ LB.disjoint const_sigma wv
-                   /\ h.[const_sigma] == Spec.const_sigma))
+    (requires (fun h -> LB.live h wv /\ LB.live h m
+                   /\ LB.disjoint wv m /\ LB.disjoint m wv))
     (ensures  (fun h0 _ h1 -> LB.modifies (LB.loc_buffer wv) h0 h1
                          /\ h1.[wv] == Spec.blake2_round h0.[m] (v i) h0.[wv]))
 
-let blake2_round wv m i const_sigma =
-  blake2_round1 wv m i const_sigma;
-  blake2_round2 wv m i const_sigma
+let blake2_round wv m i =
+  blake2_round1 wv m i;
+  blake2_round2 wv m i
 
 
-val blake2_compress1 : wv:working_vector ->
-  s:hash_state -> m:message_block_w ->
-  offset:uint64 -> flag:Spec.last_block_flag -> const_iv:iv_t ->
+val blake2_compress1:
+  wv:working_vector
+  -> s:state
+  -> m:message_block_w
+  -> offset:uint64
+  -> flag:Spec.last_block_flag ->
   Stack unit
-    (requires (fun h -> LB.live h s /\ LB.live h m /\ LB.live h wv /\ LB.live h const_iv
-                     /\ h.[const_iv] == Spec.const_iv
-                     /\ LB.disjoint wv s /\ LB.disjoint wv m /\ LB.disjoint wv const_iv
-                     /\ LB.disjoint s wv /\ LB.disjoint m wv /\ LB.disjoint const_iv wv))
+    (requires (fun h -> LB.live h s /\ LB.live h m /\ LB.live h wv
+                     /\ LB.disjoint wv s /\ LB.disjoint wv m
+                     /\ LB.disjoint s wv /\ LB.disjoint m wv))
     (ensures  (fun h0 _ h1 -> LB.modifies (LB.loc_buffer wv) h0 h1
                          /\ h1.[wv] == Spec.Blake2s.blake2_compress1 h0.[wv] h0.[s] h0.[m] offset flag))
 
 [@ Substitute ]
-let blake2_compress1 wv s m offset flag const_iv =
+let blake2_compress1 wv s m offset flag =
+  IB.recall_contents const_iv (FStar.Seq.seq_of_list Spec.list_iv);
   update_sub wv (size 0) (size 8) s;
-  update_sub wv (size 8) (size 8) const_iv;
+  assume(LB.disjoint wv const_iv);
+  update_isub wv (size 8) (size 8) const_iv;
   let low_offset = to_u32 #U64 offset in
   let high_offset = to_u32 #U64 (offset >>. u32 32) in
   // BB. Note that using the ^. operator here would break extraction !
@@ -194,300 +164,287 @@ let blake2_compress1 wv s m offset flag const_iv =
   let wv_14 = logxor #U32 wv.(size 14) (u32 0xFFFFFFFF) in
   wv.(size 12) <- wv_12;
   wv.(size 13) <- wv_13;
- (if flag then wv.(size 14) <- wv_14)
+ (if flag then wv.(size 14) <- wv_14);
+ admit()
 
 
 val blake2_compress2 :
-  wv:working_vector -> m:message_block_w -> const_sigma:sigma_t ->
+  wv:working_vector -> m:message_block_w ->
   Stack unit
-    (requires (fun h -> LB.live h wv /\ LB.live h m /\ LB.live h const_sigma
-                   /\ h.[const_sigma] == Spec.const_sigma
-                   /\ LB.disjoint wv m /\ LB.disjoint wv const_sigma
-                   /\ LB.disjoint m wv /\ LB.disjoint const_sigma wv))
+    (requires (fun h -> LB.live h wv /\ LB.live h m
+                   /\ LB.disjoint wv m /\ LB.disjoint m wv))
     (ensures  (fun h0 _ h1 -> LB.modifies (LB.loc_buffer wv) h0 h1
                          /\ h1.[wv] == Spec.blake2_compress2 h0.[wv] h0.[m]))
 
 [@ Substitute ]
-let blake2_compress2 wv m const_sigma =
+let blake2_compress2 wv m =
+  let h0 = ST.get () in
   admit();
-  (**) let h0 = ST.get () in
-  loop_nospec #h0 (size Spec.rounds_in_f) wv
-//    (fun hi -> Spec.blake2_round hi.[m])
-    (fun i -> blake2_round wv m i const_sigma)
+  loop1 #uint32 #Spec.size_block_w h0 (size Spec.rounds_in_f) wv
+    (fun h -> Spec.blake2_round h0.[m])
+    (fun i -> blake2_round wv m i)
 
 
 val blake2_compress3_inner :
-  wv:working_vector -> i:size_t{size_v i < 8} -> s:hash_state -> const_sigma:sigma_t ->
+  wv:working_vector -> i:size_t{size_v i < 8} -> s:state ->
   Stack unit
-    (requires (fun h -> LB.live h s /\ LB.live h wv /\ LB.live h const_sigma))
+    (requires (fun h -> LB.live h s /\ LB.live h wv
+                   /\ LB.disjoint s wv /\ LB.disjoint wv s))
     (ensures  (fun h0 _ h1 -> LB.modifies (LB.loc_buffer s) h0 h1
                          /\ h1.[s] == Spec.blake2_compress3_inner h0.[wv] (v i) h0.[s]))
 
 [@ Substitute ]
-let blake2_compress3_inner wv i s const_sigma =
+let blake2_compress3_inner wv i s =
   let i_plus_8 = i +. (size 8) in
   let hi_xor_wvi = s.(i) ^. wv.(i) in
-  // BB. Note that using the ^. operator here would break extraction !
   let hi = logxor #U32 hi_xor_wvi wv.(i_plus_8) in
   s.(i) <- hi
 
 
 val blake2_compress3 :
-  wv:working_vector -> s:hash_state -> const_sigma:sigma_t ->
+  wv:working_vector -> s:state ->
   Stack unit
-    (requires (fun h -> LB.live h s /\ LB.live h wv /\ LB.live h const_sigma
-                     /\ h.[const_sigma] == Spec.const_sigma
-                     /\ LB.disjoint wv s /\ LB.disjoint wv const_sigma
-                     /\ LB.disjoint s wv /\ LB.disjoint const_sigma wv))
+    (requires (fun h -> LB.live h s /\ LB.live h wv
+                     /\ LB.disjoint wv s /\ LB.disjoint s wv))
     (ensures  (fun h0 _ h1 -> LB.modifies (LB.loc_buffer s) h0 h1
                          /\ h1.[s] == Spec.blake2_compress3 h0.[wv] h0.[s]))
 
 [@ Substitute ]
-let blake2_compress3 wv s const_sigma =
+let blake2_compress3 wv s =
   admit();
-  (**) let h0 = ST.get () in
-  loop_nospec #h0 (size 8) s
-    (* (fun hi -> Spec.blake2_compress3_inner hi.[wv]) *)
-    (fun i -> blake2_compress3_inner wv i s const_sigma)
+  let h0 = ST.get () in
+  loop1 h0 (size 8) s
+    (fun h -> Spec.blake2_compress3_inner h.[wv])
+    (fun i -> blake2_compress3_inner wv i s)
 
 
 val blake2_compress :
-  s:hash_state -> m:message_block_w ->
-  offset:uint64 -> f:Spec.last_block_flag -> const_iv:iv_t -> const_sigma:sigma_t ->
+  s:state -> m:message_block_w ->
+  offset:uint64 -> f:Spec.last_block_flag ->
   Stack unit
-    (requires (fun h -> LB.live h s /\ LB.live h m /\ LB.live h const_iv /\ LB.live h const_sigma
-                         /\ h.[const_sigma] == Spec.const_sigma
-                         /\ h.[const_iv] == Spec.const_iv
-                         /\ LB.disjoint s m /\ LB.disjoint s const_sigma /\ LB.disjoint s const_iv
-                         /\ LB.disjoint m s /\ LB.disjoint const_sigma s /\ LB.disjoint const_iv s))
+    (requires (fun h -> LB.live h s /\ LB.live h m
+                     /\ LB.disjoint s m /\ LB.disjoint m s))
     (ensures  (fun h0 _ h1 -> LB.modifies (LB.loc_buffer s) h0 h1
                          /\ h1.[s] == Spec.blake2_compress h0.[s] h0.[m] offset f))
 
-let blake2_compress s m offset flag const_iv const_sigma =
-  (**) let hinit = ST.get () in
-  alloc #hinit (size 16) (u32 0) s
+let blake2_compress s m offset flag =
+  let h0 = ST.get () in
+  alloc #h0 (size 16) (u32 0) s
   (fun h0 ->
     let s0 = h0.[s] in
     let m0 = h0.[m] in
     (fun _ sv -> sv == Spec.Blake2s.blake2_compress s0 m0 offset flag))
   (fun wv ->
-    blake2_compress1 wv s m offset flag const_iv;
-    blake2_compress2 wv m const_sigma;
-    blake2_compress3 wv s const_sigma)
+    admit();
+    blake2_compress1 wv s m offset flag;
+    blake2_compress2 wv m;
+    blake2_compress3 wv s)
 
 inline_for_extraction
 val blake2s_update_block:
-    st:state
+    hash:state
   -> dd_prev:size_t{(size_v dd_prev + 1) * Spec.size_block <= max_size_t}
   -> d:message_block ->
   Stack unit
-    (requires (fun h -> state_invariant h st /\ LB.live h d
-                   /\ LB.disjoint st.hash d /\ LB.disjoint d st.hash))
-    (ensures  (fun h0 _ h1 -> LB.modifies (LB.loc_buffer st.hash) h0 h1
-                         /\ h1.[st.hash] == Spec.blake2s_update_block (v dd_prev) h0.[d] h0.[st.hash]))
+    (requires (fun h -> LB.live h hash /\ LB.live h d
+                   /\ LB.disjoint hash d /\ LB.disjoint d hash))
+    (ensures  (fun h0 _ h1 -> LB.modifies (LB.loc_buffer hash) h0 h1
+                         /\ h1.[hash] == Spec.blake2s_update_block (v dd_prev) h0.[d] h0.[hash]))
 
-let blake2s_update_block st dd_prev d =
+let blake2s_update_block hash dd_prev d =
   let h0 = ST.get () in
-  alloc #h0 (size 16) (u32 0) st.hash
-  (fun h ->
-    let d0 = h.[d] in
-    let s0 = h.[st.hash] in
+  alloc #h0 (size 16) (u32 0) hash
+  (fun h0 ->
+    let d0 = h0.[d] in
+    let s0 = h0.[hash] in
     (fun _ sv -> sv == Spec.blake2s_update_block (v dd_prev) d0 s0))
   (fun block ->
+    admit();
     uints_from_bytes_le block (size Spec.size_block_w) d;
     let offset64 = to_u64 (size_to_uint32 ((dd_prev +. (size 1)) *. (size Spec.size_block))) in
-    blake2_compress st.hash block offset64 false st.const_iv st.const_sigma
+    blake2_compress hash block offset64 false
   )
 
 val blake2s_mkstate: unit ->
   StackInline state
     (requires (fun h -> True))
-    (ensures  (fun h0 st h1 -> state_invariant h1 st
-                          /\ LB.modifies (LB.loc_union
-                                          (LB.loc_union (LB.loc_buffer st.hash) (LB.loc_buffer st.const_iv))
-                                          (LB.loc_buffer st.const_sigma)) h0 h1))
+    (ensures  (fun h0 hash h1 -> LB.live h1 hash))
 
-let blake2s_mkstate () =
-  admit();
-  {
-    hash = create (size Spec.size_hash_w) (u32 0);
-    const_iv = create_const_iv ();
-    const_sigma = create_const_sigma ();
-  }
-
+let blake2s_mkstate () = create (size Spec.size_hash_w) (u32 0)
 
 val blake2s_init_hash:
-    st:state
+    hash:state
   -> kk:size_t{v kk <= 32}
   -> nn:size_t{1 <= v nn /\ v nn <= 32} ->
   Stack unit
-     (requires (fun h -> state_invariant h st))
-     (ensures  (fun h0 _ h1 -> LB.modifies (LB.loc_buffer st.hash) h0 h1
-                          /\ h1.[st.hash] == Spec.Blake2s.blake2s_init_hash h0.[st.hash] (v kk) (v nn)))
+     (requires (fun h -> LB.live h hash))
+     (ensures  (fun h0 _ h1 -> LB.modifies (LB.loc_buffer hash) h0 h1
+                          /\ h1.[hash] == Spec.Blake2s.blake2s_init_hash h0.[hash] (v kk) (v nn)))
 
-let blake2s_init_hash st kk nn =
-  let s0 = st.hash.(size 0) in
+let blake2s_init_hash hash kk nn =
+  let s0 = hash.(size 0) in
   let kk_shift_8 = shift_left #U32 (size_to_uint32 kk) (u32 8) in
   let s0' = s0 ^. (u32 0x01010000) ^. kk_shift_8 ^. size_to_uint32 nn in
-  st.hash.(size 0) <- s0'
+  hash.(size 0) <- s0'
 
 
 val blake2s_init:
   #vkk:size_t
-  -> st:state
+  -> hash:state
   -> k:lbuffer uint8 (v vkk)
   -> kk:size_t{v kk <= 32 /\ kk == vkk}
   -> nn:size_t{1 <= v nn /\ v nn <= 32} ->
   Stack unit
-    (requires (fun h -> state_invariant h st
+    (requires (fun h -> LB.live h hash
                    /\ LB.live h k
-                   /\ LB.disjoint st.hash k /\ LB.disjoint k st.hash))
-    (ensures  (fun h0 _ h1 -> LB.modifies (LB.loc_buffer st.hash) h0 h1
-                         /\ h1.[st.hash] == Spec.Blake2s.blake2s_init (v kk) h0.[k] (v nn)))
+                   /\ LB.disjoint hash k /\ LB.disjoint k hash))
+    (ensures  (fun h0 _ h1 -> LB.modifies (LB.loc_buffer hash) h0 h1
+                         /\ h1.[hash] == Spec.Blake2s.blake2s_init (v kk) h0.[k] (v nn)))
 
 [@ Substitute ]
-let blake2s_init #vkk st k kk nn =
-  admit();
+let blake2s_init #vkk hash k kk nn =
+  IB.recall_contents const_iv (FStar.Seq.seq_of_list Spec.list_iv);
   let h0 = ST.get () in
-  alloc #h0 (size Spec.size_block) (u8 0) st.hash
+  alloc #h0 (size Spec.size_block) (u8 0) hash
   (fun h -> (fun _ sv -> sv == Spec.Blake2s.blake2s_init (v kk) h0.[k] (v nn)))
   (fun key_block ->
-    copy st.hash (size Spec.size_hash_w) st.const_iv;
-    blake2s_init_hash st kk nn;
+    admit();
+    icopy hash (size Spec.size_hash_w) const_iv;
+    blake2s_init_hash hash kk nn;
     if kk =. (size 0) then ()
     else begin
       update_sub key_block (size 0) kk k;
-      blake2s_update_block st (size 0) key_block end
+      blake2s_update_block hash (size 0) key_block end
   )
 
 
 val blake2s_update_multi_iteration:
-    st:state
+    hash:state
   -> dd_prev:size_t
   -> dd:size_t{(v dd + v dd_prev) * Spec.size_block <= max_size_t}
   -> d:lbuffer uint8 (v dd * Spec.size_block)
   -> i:size_t{v i + 1 <= v dd} ->
   Stack unit
-    (requires (fun h -> state_invariant h st
-                   /\ LB.live h d /\ LB.disjoint st.hash d /\ LB.disjoint d st.hash))
-    (ensures  (fun h0 _ h1 -> LB.modifies (LB.loc_buffer st.hash) h0 h1
-                         /\ h1.[st.hash] == Spec.blake2s_update_multi_iteration (v dd_prev) (v dd) h0.[d] (v i) h0.[st.hash]))
+    (requires (fun h -> LB.live h hash
+                   /\ LB.live h d /\ LB.disjoint hash d /\ LB.disjoint d hash))
+    (ensures  (fun h0 _ h1 -> LB.modifies (LB.loc_buffer hash) h0 h1
+                         /\ h1.[hash] == Spec.blake2s_update_multi_iteration (v dd_prev) (v dd) h0.[d] (v i) h0.[hash]))
 
 [@ Substitute ]
 let blake2s_update_multi_iteration st dd_prev dd d i =
   let block = sub d (i *. size Spec.size_block) (size Spec.size_block) in
-  blake2s_update_block st (dd_prev +. i) block
+  blake2s_update_block st (dd_prev +. i) block;
+  admit()
 
 
 val blake2s_update_multi:
-    st: state
+    hash: state
   -> dd_prev: size_t
   -> dd: size_t{(v dd + v dd_prev) * Spec.size_block <= max_size_t}
   -> d: lbuffer uint8 (size_v dd * Spec.size_block) ->
    Stack unit
-     (requires (fun h -> state_invariant h st
-                    /\ LB.live h d /\ LB.disjoint st.hash d /\ LB.disjoint d st.hash))
-     (ensures  (fun h0 _ h1 -> LB.modifies (LB.loc_buffer st.hash) h0 h1
-                          /\ h1.[st.hash] == Spec.blake2s_update_multi (v dd_prev) (v dd) h0.[d] h0.[st.hash]))
+     (requires (fun h -> LB.live h hash
+                    /\ LB.live h d /\ LB.disjoint hash d /\ LB.disjoint d hash))
+     (ensures  (fun h0 _ h1 -> LB.modifies (LB.loc_buffer hash) h0 h1
+                          /\ h1.[hash] == Spec.blake2s_update_multi (v dd_prev) (v dd) h0.[d] h0.[hash]))
 
-let blake2s_update_multi st dd_prev dd d =
+let blake2s_update_multi hash dd_prev dd d =
   admit();
-  (**) let h0 = ST.get () in
-  loop_nospec #h0 dd st.hash
-  (* (fun h -> Spec.Blake2s.blake2s_update_multi_iteration (v dd_prev) (v dd) h.[d]) *)
-  (fun i -> blake2s_update_multi_iteration st dd_prev dd d i)
-    (* Lemmas.lemma_repeati (v dd) (Spec.blake2s_update_multi_iteration (v dd_prev) (v dd) h0.[d]) h0.[st.hash] (v i)) *)
+  let h0 = ST.get () in
+  loop1 h0 dd hash
+    (fun h -> Spec.Blake2s.blake2s_update_multi_iteration (v dd_prev) (v dd) h.[d])
+    (fun i -> blake2s_update_multi_iteration hash dd_prev dd d i)
 
 
 val blake2s_update_last:
     #vlen: size_t
-  -> st: state
+  -> hash: state
   -> ll: size_t
   -> last: lbuffer uint8 (v vlen)
   -> len: size_t{v len <= Spec.size_block /\ len == vlen}
   -> flag_key: bool ->
   Stack unit
-    (requires (fun h -> state_invariant h st
-                   /\ LB.live h last /\ LB.disjoint st.hash last /\ LB.disjoint last st.hash))
-    (ensures  (fun h0 _ h1 -> LB.modifies (LB.loc_buffer st.hash) h0 h1
-                         /\ h1.[st.hash] == Spec.Blake2s.blake2s_update_last (v ll) (v len) h0.[last] flag_key h0.[st.hash]))
+    (requires (fun h -> LB.live h hash
+                   /\ LB.live h last /\ LB.disjoint hash last /\ LB.disjoint last hash))
+    (ensures  (fun h0 _ h1 -> LB.modifies (LB.loc_buffer hash) h0 h1
+                         /\ h1.[hash] == Spec.Blake2s.blake2s_update_last (v ll) (v len) h0.[last] flag_key h0.[hash]))
 
 
-let blake2s_update_last #vlen st ll last len fk =
-  admit();
+let blake2s_update_last #vlen hash ll last len fk =
   let ll64 : uint64 = to_u64 #U32 (size_to_uint32 ll) in
   let ll_plus_block_bytes64 = ll64 +. (u64 Spec.size_block) in
   assume(ll_plus_block_bytes64 == u64 (size_v ll + Spec.size_block));
   (**) let h0 = ST.get () in
-  alloc #h0 (size Spec.size_block) (u8 0) st.hash
+  alloc #h0 (size Spec.size_block) (u8 0) hash
   (fun h ->
-    let hash0 = h0.[st.hash] in
+    let hash0 = h0.[hash] in
     let last0 = h0.[last] in
     (fun _ r -> r == Spec.Blake2s.blake2s_update_last (v ll) (v len) last0 fk hash0)
   )
   (fun last_block ->
+    admit();
     update_sub last_block (size 0) len last;
     (**) let h1 = ST.get () in
-    alloc #h1 (size Spec.size_block_w) (u32 0) st.hash
+    alloc #h1 (size Spec.size_block_w) (u32 0) hash
     (fun h ->
-      let hash1 = h1.[st.hash] in
+      let hash1 = h1.[hash] in
       let last_block1 = h1.[last_block] in
       (fun _ r -> r == Spec.Blake2s.blake2s_update_last_block (v ll) last_block1 fk hash1)
     )
     (fun last_block_w ->
       uint32s_from_bytes_le last_block_w (size 16) last_block;
       if not fk then
-        blake2_compress st.hash last_block_w ll64 true st.const_iv st.const_sigma
+        blake2_compress hash last_block_w ll64 true
       else
-        blake2_compress st.hash last_block_w ll_plus_block_bytes64 true st.const_iv st.const_sigma
+        blake2_compress hash last_block_w ll_plus_block_bytes64 true
     )
   )
 
 
 val blake2s_update_last_empty:
-  st: state ->
+  hash: state ->
   Stack unit
-    (requires (fun h -> state_invariant h st))
-    (ensures  (fun h0 _ h1 -> LB.modifies (LB.loc_buffer st.hash) h0 h1
+    (requires (fun h -> LB.live h hash))
+    (ensures  (fun h0 _ h1 -> LB.modifies (LB.loc_buffer hash) h0 h1
                          /\ (let data = Seq.create Spec.size_block (u8 0) in
-                           h1.[st.hash] == Spec.Blake2s.blake2s_update_last (Spec.size_block) (Spec.size_block) data false h0.[st.hash])))
+                           h1.[hash] == Spec.Blake2s.blake2s_update_last (Spec.size_block) (Spec.size_block) data false h0.[hash])))
 
-let blake2s_update_last_empty st =
-  admit();
+let blake2s_update_last_empty hash =
   let h0 = ST.get () in
-  alloc #h0 (size Spec.size_block) (u8 0) st.hash
-  (fun h ->
-    let hash0 = h.[st.hash] in
+  alloc #h0 (size Spec.size_block) (u8 0) hash
+  (fun h0 ->
+    let hash0 = h0.[hash] in
     (fun _ r ->
       let data = Seq.create Spec.size_block (u8 0) in
       r ==  Spec.Blake2s.blake2s_update_last (Spec.size_block) (Spec.size_block) data false hash0))
   (fun data ->
-      blake2s_update_last #(size Spec.size_block) st (size Spec.size_block) data (size Spec.size_block) false
-  )
+    admit();
+    blake2s_update_last #(size Spec.size_block) hash (size Spec.size_block) data (size Spec.size_block) false)
 
 
 val blake2s_finish:
     #vnn: size_t
   -> output: lbuffer uint8 (v vnn)
-  -> st: state
+  -> hash: state
   -> nn: size_t{1 <= v nn /\ v nn <= 32 /\ nn == vnn} ->
   Stack unit
-    (requires (fun h -> state_invariant h st
-                   /\ LB.live h output /\ LB.disjoint output st.hash /\ LB.disjoint st.hash output))
+    (requires (fun h -> LB.live h hash
+                   /\ LB.live h output /\ LB.disjoint output hash /\ LB.disjoint hash output))
     (ensures  (fun h0 _ h1 -> LB.modifies (LB.loc_buffer output) h0 h1
-                         /\ h1.[output] == Spec.Blake2s.blake2s_finish h0.[st.hash] (v nn)))
+                         /\ h1.[output] == Spec.Blake2s.blake2s_finish h0.[hash] (v nn)))
 
-let blake2s_finish #vnn output s nn =
-  admit();
+let blake2s_finish #vnn output hash nn =
   (**) let h0 = ST.get () in
   alloc #h0 (size 32) (u8 0) output
   (fun h ->
-    (fun _ r -> r == Spec.Blake2s.blake2s_finish h0.[s.hash] (v nn))
+    (fun _ r -> r == Spec.Blake2s.blake2s_finish h0.[hash] (v nn))
   )
   (fun full ->
-    uints_to_bytes_le full (size 8) s.hash;
+    admit();
+    uints_to_bytes_le full (size 8) hash;
     let final = sub full (size 0) nn in
     copy output nn final)
+
 
 inline_for_extraction noextract
 val blake2s:
@@ -508,102 +465,21 @@ val blake2s:
                          /\ h1.[output] == Spec.Blake2s.blake2s (v ll) h0.[d] (v kk) h0.[k] (v nn)))
 
 let blake2s #vll #vkk #vnn output d ll k kk nn =
-  admit();
-  let st = blake2s_mkstate () in
-  let fk = if kk =. (size 0) then false else true in
-  let rem = ll %. (size Spec.size_block) in
-  let nblocks = ll /. (size Spec.size_block) in
-  let blocks = sub #_ #_ #(v nblocks * Spec.size_block) d (size 0) (nblocks *. (size Spec.size_block)) in
-  let last = sub #_ #_ #(v rem) d (nblocks *. (size Spec.size_block)) rem in
-  blake2s_init #vkk st k kk nn;
-  if ll =. (size 0) && kk =. (size 0) then blake2s_update_last_empty st
-  else begin
-    let nprev = if kk =. (size 0) then (size 0) else (size 1) in
-    blake2s_update_multi st nprev nblocks d;
-    blake2s_update_last #rem st ll last rem fk
-  end;
-  blake2s_finish #vnn output st nn
-
-
-///
-/// Experimental variant
-///
-
-(* inline_for_extraction val mkstate: *)
-(*   #h0: mem -> *)
-(*   #b: Type0 -> *)
-(*   #w: Type0 -> *)
-(*   #wlen: size_nat -> *)
-(*   write: lbuffer w wlen -> *)
-(*   spec:(h:mem -> GTot(r:b -> LSeq.lseq w (wlen) -> Type)) -> *)
-(*   impl:(st:state -> *)
-(*         Stack b *)
-(*         (requires (fun h -> state_invariant h st *)
-(* 		                 /\ preserves_live h0 h *)
-(* 		                 /\ modifies3 st.hash st.const_iv st.const_sigma h0 h)) *)
-(*         (ensures (fun h r h' -> preserves_live h h' *)
-(*                            /\ modifies2 st.hash write h h' /\ *)
-(* 			 spec h0 r (as_seq write h')))) -> *)
-(*   Stack b *)
-(*     (requires (fun h -> h == h0 /\ live h write)) *)
-(*     (ensures (fun h0 r h1 -> preserves_live h0 h1 /\ *)
-(* 		          modifies1 write h0 h1 /\ *)
-(* 		          spec h0 r (as_seq write h1))) *)
-
-(* let mkstate #h0 #b #w #wlen write spec impl = *)
-(*   admit(); *)
-(*   let h0 = ST.get () in *)
-(*   alloc #h0 (size Spec.size_hash_w) (u32 0) write *)
-(*   (fun h -> (fun _ sv -> True)) *)
-(*   (fun hash -> *)
-(*     let h0 = ST.get () in *)
-(*     alloc_with #h0 (size 8) Spec.const_iv create_const_iv write *)
-(*     (fun h -> (fun _ _ -> True)) *)
-(*     (fun const_iv -> *)
-(*       let h0 = ST.get () in *)
-(*       alloc_with #h0 (size 160) Spec.const_sigma create_const_sigma write *)
-(*       (fun h -> (fun _ _ -> True)) *)
-(*       (fun const_sigma -> *)
-(*         let st = {hash = hash; const_iv = const_iv; const_sigma = const_sigma} in *)
-(*         impl st *)
-(*       ) *)
-(*     ) *)
-(*   ) *)
-
-
-(* val blake2s: *)
-(*     #vll: size_t *)
-(*   -> #vkk: size_t *)
-(*   -> #vnn: size_t *)
-(*   -> output: lbuffer uint8 (v vnn) *)
-(*   -> d: lbuffer uint8 (v vll) *)
-(*   -> ll: size_t{v ll + 2 * Spec.size_block <= max_size_t /\ ll == vll} // This could be relaxed *)
-(*   -> k: lbuffer uint8 (v vkk) *)
-(*   -> kk: size_t{v kk <= 32 /\ kk == vkk} *)
-(*   -> nn:size_t{1 <= v nn /\ v nn <= 32 /\ nn == vnn} -> *)
-(*   Stack unit *)
-(*     (requires (fun h -> live h output /\ live h d /\ live h k *)
-(*                    /\ LB.disjoint output d /\ LB.disjoint d output *)
-(*                    /\ LB.disjoint output k /\ LB.disjoint k output)) *)
-(*     (ensures  (fun h0 _ h1 -> preserves_live h0 h1 /\ modifies1 output h0 h1 *)
-(*                          /\ h1.[output] == Spec.Blake2s.blake2s (v ll) h0.[d] (v kk) h0.[k] (v nn))) *)
-
-(* let blake2s #vll #vkk #vnn output d ll k kk nn = *)
-(*   let h0 = ST.get () in *)
-(*   mkstate #h0 output *)
-(*   (fun h -> (fun _ sv -> sv == Spec.Blake2s.blake2s (v ll) h0.[d] (v kk) h0.[k] (v nn))) *)
-(*   (fun st -> *)
-(*     let fk = if kk =. (size 0) then false else true in *)
-(*     let rem = ll %. (size Spec.size_block) in *)
-(*     let nblocks = ll /. (size Spec.size_block) in *)
-(*     let blocks = sub #_ #_ #(v nblocks * Spec.size_block) d (size 0) (nblocks *. (size Spec.size_block)) in *)
-(*     let last = sub #_ #_ #(v rem) d (nblocks *. (size Spec.size_block)) rem in *)
-(*     blake2s_init #vkk st k kk nn; *)
-(*     if ll =. (size 0) && kk =. (size 0) then blake2s_update_last_empty st *)
-(*     else begin *)
-(*       let nprev = if kk =. (size 0) then (size 0) else (size 1) in *)
-(*       blake2s_update_multi st nprev nblocks d; *)
-(*       blake2s_update_last #rem st ll last rem fk *)
-(*     end; *)
-(*     blake2s_finish #vnn output st nn *)
-(*   ) *)
+  let h0 = ST.get () in
+  alloc #h0 (size 8) (u32 0) output
+  (fun h -> (fun _ r -> r == Spec.Blake2s.blake2s (v ll) h0.[d] (v kk) h0.[k] (v nn)))
+  (fun hash ->
+    let fk = if kk =. (size 0) then false else true in
+    let rem = ll %. (size Spec.size_block) in
+    let nblocks = ll /. (size Spec.size_block) in
+    let blocks = sub #_ #_ #(v nblocks * Spec.size_block) d (size 0) (nblocks *. (size Spec.size_block)) in
+    let last = sub #_ #_ #(v rem) d (nblocks *. (size Spec.size_block)) rem in
+    admit();
+    blake2s_init #vkk hash k kk nn;
+    if ll =. (size 0) && kk =. (size 0) then blake2s_update_last_empty hash
+    else begin
+      let nprev = if kk =. (size 0) then (size 0) else (size 1) in
+      blake2s_update_multi hash nprev nblocks d;
+      blake2s_update_last #rem hash ll last rem fk
+    end;
+    blake2s_finish #vnn output hash nn)
